nola/examples/later.v
@@ -48,7 +48,7 @@ Section iris.
     rewrite ilist_unfold. iDestruct "l" as "[ihd itl]". wp_rec. wp_pures.
     wp_load. wp_pures. wp_apply "Hf"; [done|]. iIntros "_". wp_pures. wp_load.
     wp_op. have -> : (S m - 1)%Z = m by lia. wp_store. wp_op. wp_bind (! _)%E.
-    iMod (inv_tok_acc (PROP:=▶ ∙) (intp:=laterl) with "itl") as
+    iMod (inv_tok_acc (PROP:=▶ ∙) (ip:=laterl) with "itl") as
       "/=[(%l' & ↦l' & #l') cl]"; [done|].
     wp_load. iModIntro. iMod ("cl" with "[↦l']") as "_".
     { iNext. iExists _. by iFrame "↦l'". }
